Heap/test.v
@@ -1,0 +1,8 @@
+Require Import PL.Monad.
+Require Import PL.Monad.
+Import SetsNotation
+       KleeneFix Sets_CPO
+       Monad
+       MonadNotation.
+
+Check bind.
