README.md
@@ -1,1 +1,15 @@
 # CS2205-CoqProject
+
+### 编译
+
+- 先配置 `CONFIGURE` 文件（如果需要），然后：
+```
+> make depend
+> make
+```
+
+
+    
+
+
+
